{\bf Part 1: Two Fibonaccis}

$fib(n):$
\begin{algorithmic}
\IF { $ n=0 $ or $ n=1 $ }
\RETURN $n$
\ELSE
\RETURN $fib(n-1) + fib(n-2)$
\ENDIF
\end{algorithmic}

We can state a recurrence for this algorithm:

\begin{align*}
T(n) 
&= T(n-1) + T(n-2) + O(1) \\
&\geq fib(n-1) + fib(n-2) \\
&= fib(n)
\end{align*}

$fib2(n):$
\begin{algorithmic}
\IF { $ n = 0 $ }
\RETURN 0
\ENDIF
\STATE create array $f[0 .. n]$
\STATE $f[0] \leftarrow 0, f[1] \leftarrow 1$
\FOR { $ i \leftarrow 2$ to $n$ }
\STATE $f[i] \leftarrow f[i-1] + f[i-2]$
\ENDFOR
\RETURN $f[n]$
\end{algorithmic}

Addition of two numbers in the preceding algorithm takes constant time
until the values exceed the maximum value that can be stored in a
word.  After which, we need to consider how values of arbitrary length
are added.
