\chapter{Integer Multiplication}

Let us consider an integer $X$ which is composed of $X_L$ which are
the leftmost bits of $X$, and $X_R$ which are the rightmost bits of
$X$.

\begin{displaymath}
X = X_L | X_R
\end{displaymath}

We can multiply integers $X,Y$ as follows:

\begin{align*}
XY
&= (2^{n/2}X_L + X_R)(2^{n/2}Y_L + Y_R) \\
&= 2^n X_LY_L + 2^{n/2}X_LY_R + 2^{n/2}X_RY_L + X_RY_R \\
&= 2^n X_LY_L + 2^{n/2}(X_LY_R + X_RY_L) + X_RY_R \\
\end{align*}

Which gives the recurrence

\begin{align*}
T(n)
&= 4T(n/2) + O(n) \\
&\leq 4T(n/2) + cn \\
&\leq 4(4T(n/4) + cn/2) + cn \\
&\leq 4(4(4T(n/8) + cn/4) + cn/2) + cn \\
&\leq 64T(n/8) + cn(1 + 2 + 4) \\
&... \\
&\leq 4^iT(n/2^i) + cn(1 + 2 + ... + 2^{i-1})
\end{align*}

Where $i$ is the number of times we can divide $n$ by 2, or $log_2n$.

\begin{align*}
T(n)
&\leq 4^{log_2n}T(n/2^{log_2n}) + cn(1 + 2 + ... + 2^{log_2n-1}) \\
&\leq n^{log_24}T(n/n^{log_22}) + cn \sum\limits_{i=0}^{log_2n-1} 2^i \\
&\leq n^2T(1) + cn 2^{log_2n} \\
&\leq n^2T(1) + cn n^{log_22} \\
&\leq n^2T(1) + cn^2 \\
&\leq n^2(T(1) + c) \\
&\leq n^2(O(1) + c) \\
&\leq O(n^2)
\end{align*}

Can we do better?  Turns out: yes.

We need: $X_LY_L, X_RY_R,$ and $X_LY_R + X_RY_L$

Observe: 
%
\begin{align*}
&(X_L + X_R)(Y_L + Y_R) - X_LY_L - X_RY_R \\
&= X_LY_L + X_RY_L + X_LY_R + X_RY_R - X_LY_L - X_RY_R \\
&= X_RY_L + X_LY_R
\end{align*}

Since we must compute $X_LY_L$ and $X_RY_R$ anyway, this saves us an
entire multiplication.  Reducing our recurrence from $T(n) = 4T(n/2) +
O(n)$ to $T(n) = 3T(n/2) + O(n)$.

We can solve this new recurrence as follows:

\begin{align*}
T(n)
&= 3T(n/2) + O(n) \\
&\leq 3T(n/2) + cn \\
&\leq 3(3T(n/4) + cn/2) + cn \\
&\leq 3^iT(n/2^i) + cn(1 + 3/2 + ... + (3/2)^{i-1}) \\
&\leq 3^{log_2n}T(n/2^{log_2n}) + cn(1 + 2 + ... + (3/2)^{log_2n-1}) \\
&\leq n^{log_23}T(1) + cn \sum\limits_{i=0}^{log_2n-1} (3/2)^i \\
&\leq n^{log_23}T(1) + cn (3/2)^{log_2n} \\
&\leq n^{log_23}T(1) + cn n^{log_2(3/2)} \\
&\leq n^{log_23}T(1) + cn n^{log_23 - log_22} \\
&\leq n^{log_23}T(1) + cn n^{log_23 - 1} \\
&\leq n^{log_23}T(1) + cn n^{log_23}n^{-1} \\
&\leq n^{log_23}(T(1) + cn/n) \\
&\leq n^{log_23}(T(1) + c) \\
&\leq O(n^{log_23})
\end{align*}
